compcertox/TensorComp.v
@@ -25,46 +25,41 @@ Section APPLY.
   Context {liA1 liA2 liB1 liB2 S} (L: lts liA1 liB1 S)
           (FA: li_func liA1 liA2) (FB: li_func liB1 liB2).
 
-  Definition lts_map_outgoing: lts liA1 liB2 S :=
+  Definition lts_map: lts liA2 liB2 S :=
     {|
       genvtype := genvtype L;
       globalenv := globalenv L;
       step := step L;
       initial_state q s := initial_state L (query_func FB q) s;
-      at_external := at_external L;
-      after_external := after_external L;
-      final_state s r := final_state L s (reply_func FB r);
-    |}.
-
-  Definition lts_map_incoming: lts liA2 liB1 S :=
-    {|
-      genvtype := genvtype L;
-      globalenv := globalenv L;
-      step := step L;
-      initial_state := initial_state L;
       at_external s q := at_external L s (query_func FA q);
       after_external s r s' := after_external L s (reply_func FA r) s';
-      final_state := final_state L;
+      final_state s r := final_state L s (reply_func FB r);
     |}.
 
 End APPLY.
 
-Definition map_outgoing {liA liB1 liB2} (L: semantics liA liB1) (F: li_func liB1 liB2) :=
+Definition semantics_map {liA1 liA2 liB1 liB2} (L: semantics liA1 liB1)
+           (F: li_func liA1 liA2) (G: li_func liB1 liB2) :=
   {|
     skel := skel L;
-    activate se := lts_map_outgoing (L se) F;
+    activate se := lts_map (L se) F G;
     footprint := footprint L;
   |}.
 
+Definition id_li_func {liA} := mk_li_func liA liA id id.
+
+Definition map_outgoing {liA liB1 liB2} (L: semantics liA liB1) (F: li_func liB1 liB2) :=
+  semantics_map L id_li_func F.
+
 Definition map_incoming {liA1 liA2 liB} (L: semantics liA1 liB) (F: li_func liA1 liA2) :=
-  {|
-    skel := skel L;
-    activate se := lts_map_incoming (L se) F;
-    footprint := footprint L;
-  |}.
+  semantics_map L F id_li_func.
+
+Definition map_both {li1 li2} (L: semantics li1 li1) (F: li_func li1 li2) :=
+  semantics_map L F F.
 
 Infix "##" := map_incoming (at level 50): lts_scope.
 Infix "$$" := map_outgoing (at level 50): lts_scope.
+Infix "%%" := map_both (at level 50): lts_scope.
 
 (* The generated definition looks funky
    Try use idtac as default *)
@@ -80,30 +75,121 @@ Program Definition li_func_k {li K1 K2}: li_func ((li@K1)@K2) (li@(K1*K2)) :=
     reply_func '(r, k) := ((r, fst k), snd k);
   |}.
 
+Program Definition li_func_comm {li K1 K2}: li_func (li@(K1*K2)) (li@(K2*K1)) :=
+  {|
+    query_func '(q, (k1, k2)) := (q, (k2, k1));
+    reply_func '(r, (k1, k2)) := (r, (k2, k1));
+  |}.
+
 Definition lift_layer {li K} (L: semantics li_null li): semantics li_null (li@K) :=
   L@K ## li_func_null.
 
 Definition lift_layer_k {li K1 K2} (L: semantics li_null (li@K1)): semantics li_null (li@(K1*K2)) :=
   L@K2 ## li_func_null $$ li_func_k.
 
-Infix "⊗" := kcc_tensor (at level 50, left associativity) : cc_scope.
+Definition layer_comm {li K1 K2} (L: semantics li_null (li@(K2*K1))): semantics li_null (li@(K1*K2)) :=
+  L $$ li_func_comm.
+
+Definition lts_comm {li K1 K2} (L: semantics (li@(K2*K1)) (li@(K2*K1))): semantics (li@(K1*K2)) (li@(K1*K2)) :=
+  L %% li_func_comm.
+
+Section Properties.
+
+  Context {K1 K2 K3 K4} (R1: krel K1 K2) (R2: krel K3 K4).
+  Lemma prod_match_reply w r1 r2 k1 k2 k3 k4:
+    match_reply R1 w (r1, k1) (r2, k2) ->
+    Rk R2 k3 k4 -> Rr R2 k3 (cr_mem r2) ->
+    (* kmrel (krel_crel R2) (cr_mem r1, k3) (cr_mem r2, k4) -> *)
+    match_reply (R1 * R2) w (r1, (k1, k3)) (r2, (k2, k4)).
+  Proof.
+    intros [w' [Hw' Hr]] H. exists w'; split.
+    - cbn in *. eapply Mem.unchanged_on_implies; eauto.
+      cbn in *. intros. intro contra. apply H1. now left.
+    - inv Hr. cbn in *. constructor; eauto.
+      + split; eauto.
+      + split; eauto.
+  Qed.
+
+  Lemma prod_match_query w q1 q2 k1 k2 k3 k4:
+    match_query (R1 * R2) w (q1, (k1, k3)) (q2, (k2, k4)) ->
+    match_query R1 w (q1, k1) (q2, k2) /\ Rk R2 k3 k4 /\ Rr R2 k3 w.
+  Proof.
+    intros. inv H. repeat apply conj; cbn in *.
+    constructor; eauto.
+    - intros b ofs Hg. apply H9. now left.
+    - firstorder.
+    - firstorder.
+    - firstorder.
+    - firstorder.
+  Qed.
+
+End Properties.
 
 Section TENSOR.
 
   Context {K1 K2} (L1: semantics li_null (li_c@K1)) (L2: semantics li_null (li_c@K2)).
-  Context {J1 J2} (jcc: crel J1 J2) (kcc: callconv (li_c@K1) (li_c@K2)).
+  Context {J1 J2} (jcc: krel J1 J2) (kcc: krel K1 K2).
   Context (HL: fsim_components 1 kcc L1 L2).
+  Context (se1 se2: Genv.symtbl) (w : ccworld (kcc * jcc)).
+  Context (Hse: match_senv (kcc * jcc) w se1 se2).
+  Context (Hse1: Genv.valid_for (skel L1) se1).
 
-  (* One more condition we need from crel maybe match_query implies match_reply
-     if the memory is unchanged on the blocks in the crel *)
+  Hypothesis Hdisjoint: forall b ofs, G jcc b ofs -> G kcc b ofs -> False.
 
-  Inductive state_match:
+  Inductive state_match: fsim_index HL -> state L1 * J1 -> state L2 * J2 -> Prop :=
+  | lift_state_match i s1 j1 s2 j2:
+      fsim_match_states HL se1 se2 w i s1 s2 ->
+      Rk jcc j1 j2 -> Rr jcc j1 w ->
+      state_match i (s1, j1) (s2, j2).
 
-  Lemma lift_layer_fsim: forward_simulation 1 (kcc ⊗ jcc) (lift_layer_k L1) (lift_layer_k L2).
+  Lemma lift_layer_semantics_simulation:
+    fsim_properties 1 (kcc * jcc) se1 se2 w
+      (lift_layer_k L1 se1) (lift_layer_k L2 se2)
+      (fsim_index HL) (fsim_order HL) state_match.
   Proof.
-
+    split; cbn.
+    - intros [q1 [k1 j1]] [q2 [k2 j2]] [s1 sj1] Hq [H Hj]; cbn in *.
+      subst sj1. eapply prod_match_query in Hq.
+      pose proof (fsim_lts HL _ w Hse Hse1).
+      edestruct @fsim_match_initial_states as (idx & s2 & Hs2 & Hs); eauto.
+      apply Hq. exists idx, (s2, j2). split. split; auto.
+      constructor; auto. apply Hq. apply Hq.
+    - intros idx [s1 sj1] [s2 sj2] [r1 [kr1 jr1]] Hs [H Hj].
+      inv Hs. pose proof (fsim_lts HL _ w Hse Hse1).
+      edestruct @fsim_match_final_states as (r2 & Hr2 & Hr); eauto.
+      cbn [fst snd] in *. destruct r2 as [r2 rk2]. subst sj1.
+      exists (r2, (rk2, sj2)). split. split; eauto.
+      apply prod_match_reply. apply Hr. auto.
+      eapply G_unchanged; eauto.
+      destruct Hr as [w' [Hw' Hr]]. inv Hr.
+      eapply Mem.unchanged_on_implies. apply Hw'.
+      cbn. intros. intros contra. eapply Hdisjoint; eauto.
+    - intros i [s1 sj1] [s2 sj2] [ ].
+    - intros [s1 sj1] t [s1' sj1'] H idx [s2 sj2] Hs. destruct H as [H <-].
+      inv Hs. pose proof (fsim_lts HL _ w Hse Hse1).
+      edestruct @fsim_simulation as (idx' & s2' & Hs2' & Hs'); eauto.
+      exists idx', (s2', sj2). split.
+      + destruct Hs2'; [left | right].
+        apply lifting_step_plus; eauto.
+        split. apply lifting_step_star; eauto. intuition. intuition.
+      + constructor; eauto.
+  Qed.
 
 End TENSOR.
+
+Lemma layer_lifting_simulation {K1 K2 J1 J2} (kcc: krel K1 K2) (jcc: krel J1 J2) L1 L2:
+  (forall b ofs, G jcc b ofs -> G kcc b ofs -> False) -> forward_simulation 1 kcc L1 L2 ->
+  forward_simulation 1 (kcc * jcc) (lift_layer_k L1) (lift_layer_k L2).
+Proof.
+  intros Hdisjoint [HL]. constructor.
+  eapply Forward_simulation with (fsim_order HL) (state_match L1 L2 jcc kcc HL).
+  - eapply (fsim_skel HL).
+  - intros. apply (fsim_footprint HL i).
+  - intros. eapply lift_layer_semantics_simulation; eauto.
+  - apply (fsim_order_wf HL).
+Qed.
+
+
 
 Class mem_ops: Type :=
   {
